Suncraft

Gt3/HasTy/Inversion.lean
@@ -1,5 +1,14 @@
 import Gt3.HasTy.Regular
 
+def Ctx.HasTyUnder (Γ : Ctx) (A : Tm 0) (B b : Tm 1) : Prop
+  := ∀ x ∉ Γ.dv, HasTy (Γ.cons x A) (B.open x) (b.open x)
+
+def Ctx.IsWfUnder (Γ : Ctx) (A : Tm 0) (B : Tm 1) : Prop
+  := ∀ x ∉ Γ.dv, IsWf (Γ.cons x A) (B.open x)
+
+def Ctx.IsTyUnder (Γ : Ctx) (A : Tm 0) (B : Tm 1) : Prop
+  := ∀ x ∉ Γ.dv, IsTy (Γ.cons x A) (B.open x)
+
 theorem Ctx.HasTy.exists_pi_arg_general {Γ U A B P} (h : HasTy Γ U P) (hP : P = .pi A B)
   : ∃ℓ, HasTy Γ (.univ ℓ) A := by induction h with
   | pi hA => cases hP; exact ⟨_, hA⟩
@@ -16,6 +25,13 @@ theorem Ctx.HasTy.exists_pi_arg {Γ U A B} (h : HasTy Γ U (.pi A B))
 theorem Ctx.HasTy.exists_pi_res {Γ U A B} (h : HasTy Γ U (.pi A B))
   : ∃ℓ, ∀ x ∉ Γ.dv, HasTy (Γ.cons x A) (.univ ℓ) (B.open x) := exists_pi_res_general h rfl
 
+theorem Ctx.IsWf.exists_pi_arg {Γ A B} (h : IsWf Γ (.pi A B))
+  : ∃ℓ, HasTy Γ (.univ ℓ) A := have ⟨_, h⟩ := h.has_ty; h.exists_pi_arg
+
+theorem Ctx.IsWf.exists_pi_res {Γ A B} (h : IsWf Γ (.pi A B))
+  : ∃ℓ, ∀ x ∉ Γ.dv, HasTy (Γ.cons x A) (.univ ℓ) (B.open x)
+  := have ⟨_, h⟩ := h.has_ty; h.exists_pi_res
+
 theorem Ctx.HasTy.exists_sigma_arg_general {Γ U A B P} (h : HasTy Γ U P) (hP : P = .sigma A B)
   : ∃ℓ, HasTy Γ (.univ ℓ) A := by induction h with
   | sigma hA => cases hP; exact ⟨_, hA⟩
@@ -31,6 +47,13 @@ theorem Ctx.HasTy.exists_sigma_arg {Γ U A B} (h : HasTy Γ U (.sigma A B))
 
 theorem Ctx.HasTy.exists_sigma_res {Γ U A B} (h : HasTy Γ U (.sigma A B))
   : ∃ℓ, ∀ x ∉ Γ.dv, HasTy (Γ.cons x A) (.univ ℓ) (B.open x) := exists_sigma_res_general h rfl
+
+theorem Ctx.IsWf.exists_sigma_arg {Γ A B} (h : IsWf Γ (.sigma A B))
+  : ∃ℓ, HasTy Γ (.univ ℓ) A := have ⟨_, h⟩ := h.has_ty; h.exists_sigma_arg
+
+theorem Ctx.IsWf.exists_sigma_res {Γ A B} (h : IsWf Γ (.sigma A B))
+  : ∃ℓ, ∀ x ∉ Γ.dv, HasTy (Γ.cons x A) (.univ ℓ) (B.open x)
+  := have ⟨_, h⟩ := h.has_ty; h.exists_sigma_res
 
 theorem Ctx.HasTy.regular_pi_arg_ty {Γ A B f} (h : HasTy Γ (.pi A B) f)
   : ∃ℓ, HasTy Γ (.univ ℓ) A := have ⟨_, h⟩ := h.regular.has_ty; h.exists_pi_arg
@@ -104,3 +127,106 @@ theorem Ctx.IsWf.trunc {Γ A} (h : IsTy Γ A) : IsWf Γ (.trunc A)
 
 theorem Ctx.IsWf.trunc_wf_iff {Γ A} : IsWf Γ (.trunc A) ↔ IsTy Γ A
   := ⟨trunc_is_ty, trunc⟩
+
+theorem Ctx.HasTy.exists_app_general {Γ U f a P} (h : HasTy Γ U P) (hP : P = .app f a)
+  : ∃A B, HasTy Γ (.pi A B) f ∧ HasTy Γ A a := by induction h with
+  | app' _ _ hf ha _ => cases hP; exact ⟨_, _, hf, ha⟩
+  | _ => cases hP <;> apply_assumption <;> rfl
+
+theorem Ctx.HasTy.exists_app {Γ U f a} (h : HasTy Γ U (.app f a))
+  : ∃A B, HasTy Γ (.pi A B) f ∧ HasTy Γ A a := exists_app_general h rfl
+
+theorem Ctx.HasTy.exists_abs_general {Γ U A b P} (h : HasTy Γ U P) (hP : P = .abs A b)
+  : ∃B : Tm 1, ∀ x ∉ Γ.dv, HasTy (Γ.cons x A) (B.open x) (b.open x) := by
+  induction h with
+  | abs' hA _ hb => cases hP; exact ⟨_, HasTy.top_quant_exact hb⟩
+  | _ => cases hP <;> apply_assumption <;> rfl
+
+theorem Ctx.HasTy.exists_abs {Γ U A b} (h : HasTy Γ U (.abs A b))
+  : ∃B : Tm 1, HasTyUnder Γ A B b
+  := exists_abs_general h rfl
+
+theorem Ctx.IsWf.exists_abs {Γ A b} (h : IsWf Γ (.abs A b))
+  : ∃B : Tm 1, HasTyUnder Γ A B b
+  := have ⟨_, h⟩ := h.has_ty; h.exists_abs
+
+theorem Ctx.HasTy.exists_fst_general {Γ U p P} (h : HasTy Γ U P) (hp : P = .fst p)
+  : ∃A B, HasTy Γ (.sigma A B) p := by induction h with
+  | fst' _ _ hp => cases hp; exact ⟨_, _, hp⟩
+  | _ => cases hp <;> apply_assumption <;> rfl
+
+theorem Ctx.HasTy.exists_fst {Γ U p} (h : HasTy Γ U (.fst p))
+  : ∃A B, HasTy Γ (.sigma A B) p := exists_fst_general h rfl
+
+theorem Ctx.HasTy.exists_snd_general {Γ U p P} (h : HasTy Γ U P) (hp : P = .snd p)
+  : ∃A B, HasTy Γ (.sigma A B) p := by induction h with
+  | snd' _ _ hp => cases hp; exact ⟨_, _, hp⟩
+  | _ => cases hp <;> apply_assumption <;> rfl
+
+theorem Ctx.HasTy.exists_snd {Γ U p} (h : HasTy Γ U (.snd p))
+  : ∃A B, HasTy Γ (.sigma A B) p := exists_snd_general h rfl
+
+theorem Ctx.IsWf.exists_fst {Γ p} (h : IsWf Γ (.fst p)) : ∃A B, HasTy Γ (.sigma A B) p
+  := have ⟨_, h⟩ := h.has_ty; h.exists_fst
+
+theorem Ctx.IsWf.exists_snd {Γ p} (h : IsWf Γ (.snd p)) : ∃A B, HasTy Γ (.sigma A B) p
+  := have ⟨_, h⟩ := h.has_ty; h.exists_snd
+
+theorem Ctx.IsWf.of_fst {Γ p} (h : IsWf Γ (.fst p)) : IsWf Γ p
+  := have ⟨_, _, h⟩ := h.exists_fst; h.is_wf
+
+theorem Ctx.IsWf.of_snd {Γ p} (h : IsWf Γ (.snd p)) : IsWf Γ p
+  := have ⟨_, _, h⟩ := h.exists_snd; h.is_wf
+
+theorem Ctx.HasTy.exists_pair_general {Γ U a b P} (h : HasTy Γ U P) (hP : P = .pair a b)
+  : ∃A, ∃ B : Tm 1, IsTyUnder Γ A B ∧ HasTy Γ A a ∧ HasTy Γ (B.lst a) b := by
+  induction h with
+  | pair' hA hB ha hb =>
+    cases hP;
+    exact ⟨_, _, (fun x hx => (HasTy.top_quant_exact_k hB x hx).is_ty), ha, hb⟩
+  | _ => cases hP <;> apply_assumption <;> rfl
+
+theorem Ctx.HasTy.exists_pair {Γ U a b} (h : HasTy Γ U (.pair a b))
+  : ∃A, ∃ B : Tm 1, IsTyUnder Γ A B ∧ HasTy Γ A a ∧ HasTy Γ (B.lst a) b
+  := exists_pair_general h rfl
+
+theorem Ctx.IsWf.exists_pair {Γ a b} (h : IsWf Γ (.pair a b))
+  : ∃A, ∃ B : Tm 1, IsTyUnder Γ A B ∧ HasTy Γ A a ∧ HasTy Γ (B.lst a) b
+  := have ⟨_, h⟩ := h.has_ty; h.exists_pair
+
+theorem Ctx.JEq.fst {Γ} {A : Tm 0} {B : Tm 1} {p p' : Tm 0}
+    (hp : JEq Γ (.sigma A B) p p')
+    : JEq Γ A (p.fst) (p'.fst) :=
+    have ⟨_, hA⟩ := hp.regular.wf.exists_sigma_arg;
+    have ⟨_, hB⟩ := hp.regular.wf.exists_sigma_res;
+    .fst' (fun x hx => (hB x hx).refl) hA.refl hp
+
+theorem Ctx.JEq.snd {Γ} {A : Tm 0} {B : Tm 1} {p p' : Tm 0}
+    (hp : JEq Γ (.sigma A B) p p')
+    : JEq Γ (B.lst (p.fst)) (p.snd) (p'.snd) :=
+    have ⟨_, hA⟩ := hp.regular.wf.exists_sigma_arg;
+    have ⟨_, hB⟩ := hp.regular.wf.exists_sigma_res;
+    .snd' (fun x hx => (hB x hx).refl) hA.refl hp
+      (.lst_cf₁_k (fun x hx => (hB x hx).refl) (.fst hp.lhs_ty'))
+
+theorem Ctx.JEq.beta_fst_both {Γ} {A : Tm 0} {B : Tm 1} {a b : Tm 0} {L : Finset String}
+    (hB : ∀ x ∉ L, IsTy (Γ.cons x A) (B.open x))
+    (ha : HasTy Γ A a) (hb : HasTy Γ (B.lst a) b)
+    : JEq Γ A (.fst (.pair a b)) a
+    :=
+    have ⟨_, hA⟩ := ha.regular;
+    have ⟨_, hB⟩ := IsTy.max_univ' hB;
+    have hpair := (JEq.pair' hB hA ha.refl hb.refl)
+    .beta_fst' hA hB hpair (.fst hpair) ha.refl
+
+theorem Ctx.JEq.beta_snd_both {Γ} {A : Tm 0} {B : Tm 1} {a b : Tm 0} {L : Finset String}
+    (hB : ∀ x ∉ L, IsTy (Γ.cons x A) (B.open x))
+    (ha : HasTy Γ A a) (hb : HasTy Γ (B.lst a) b)
+    : JEq Γ (B.lst a) (.snd (.pair a b)) b
+    :=
+    have ⟨_, hA⟩ := ha.regular;
+    have ⟨_, hB'⟩ := IsTy.max_univ' hB;
+    have hfst := JEq.beta_fst_both hB ha hb
+    have hpair := (JEq.pair' hB' hA ha.refl hb.refl)
+    (JEq.beta_snd' hA hB' hpair (.snd hpair) (hb.lst_cast hB' hfst.symm).refl).cast
+      (TyEq.lst_cf hB hfst)
